sha3/proof/AbsorbToBlocks.ec
@@ -5,7 +5,6 @@ require (*--*) Absorb Blocks.
 (* -------------------------------------------------------------------- *)
 require import Common.
 
-op ( * ): 'a NewDistr.distr -> 'b NewDistr.distr -> ('a * 'b) distr.
 op cast: 'a NewDistr.distr -> 'a distr.
 
 op extend (bs : block list) (n : int): block list =
@@ -20,6 +19,19 @@ op strip_aux (bs : block list) (n : int) : block list * int =
 
 op strip (bs : block list) = strip_aux (rev bs) 0.
 
+lemma ge0_strip_aux n bs:
+  0 <= n =>
+  0 <= (strip_aux bs n).`2.
+proof.
+  elim bs n=> //= b bs ih n le0_n.
+  case (b = b0)=> //=.
+  by rewrite (ih (n + 1) _) 1:smt.
+qed.
+
+lemma ge0_strip2 bs:
+  0 <= (strip bs).`2.
+proof. by rewrite /strip; exact/(ge0_strip_aux 0 (rev bs)). qed.
+
 op valid_upper (bs : block list) =
   bs <> [] /\
   forallb (fun n=> strip (extend bs n) = (bs,n)).
@@ -29,12 +41,10 @@ op valid_lower (bs : block list) =
 
 (* PY: FIXME *)
 clone Absorb as Lower with
-  op ( * ) <- ( * )<:'a,'b>,
   op cast  <- cast<:'a>,
   op valid <- valid_lower.
 
 clone Blocks as Upper with
-  op ( * ) <- ( * )<:'a,'b>,
   op valid <- valid_upper.
 
 (* -------------------------------------------------------------------- *)
@@ -80,57 +90,200 @@ module UpperOfLowerBlockSponge (P : Upper.PRIMITIVE) = UpperFun(Lower.BlockSpong
 module Dist ( D : Upper.DISTINGUISHER, F : Lower.FUNCTIONALITY, P : Lower.PRIMITIVE ) = D(UpperFun(F),P).
 
 section.
-  declare module LowerSim  : Lower.SIMULATOR.
-  declare module UpperDist : Upper.DISTINGUISHER { LowerSim }.
+  declare module LowerSim  : Lower.SIMULATOR { Perm, Upper.BIRO.IRO', Lower.Ideal.RO }.
+  declare module UpperDist : Upper.DISTINGUISHER { Perm, Upper.BIRO.IRO', Lower.Ideal.RO, LowerSim }.
 
-  local equiv ModularUpper:
-    UpperFun(Lower.BlockSponge(Lower.Perm.Perm)).f ~ Upper.BlockSponge(Upper.Perm.Perm).f:
+  local equiv ModularUpper_Real:
+    UpperFun(Lower.BlockSponge(Perm)).f ~ Upper.BlockSponge(Perm).f:
          ={arg}
-      /\ ={m,mi}(Lower.Perm.Perm,Upper.Perm.Perm)
-      /\ (forall x, mem (dom Lower.Perm.Perm.m){1} x)
+      /\ ={m,mi}(Perm,Perm)
+      /\ (forall x, mem (dom Perm.m){1} x)
       ==>    ={res}
-          /\ ={m,mi}(Lower.Perm.Perm,Upper.Perm.Perm)
-          /\ (forall x, mem (dom Lower.Perm.Perm.m){1} x).
+          /\ ={m,mi}(Perm,Perm)
+          /\ (forall x, mem (dom Perm.m){1} x).
   proof.
   proc. sp; if=> //=.
-  inline Lower.BlockSponge(Lower.Perm.Perm).f.
+  inline Lower.BlockSponge(Perm).f.
   admit. (* Fun with loops *)
   qed.
 
-  pred relation (ro : (block list,block) fmap) (iro : (block list,block list) fmap) =
-    (forall x y, iro.[x] = Some y =>
-      forall i, 0 <= i < size y => ro.[extend x i] = onth y i)
- /\ (forall x y, ro.[x] = Some y =>
-      let (x',n) = strip x in
-         mem (dom iro) x
-      /\ size (oget iro.[x]) >= n
-      /\ nth witness (oget iro.[x]) n = y).
+  pred lower (ro : (block list,block) fmap) (iro : (block list * int,block) fmap) =
+    Upper.BIRO.prefix_closed iro /\
+    forall x n, valid_upper x => iro.[(x,n)] = ro.[extend x n].
 
   local equiv ModularLower:
-    UpperFun(Lower.Ideal.RO).f ~ Upper.BIRO.IRO.f:
+    UpperFun(Lower.Ideal.RO).f ~ Upper.BIRO.IRO'.f:
           ={arg}
-          /\ relation Lower.Ideal.RO.m{1} Upper.BIRO.IRO.mp{2}
+          /\ lower Lower.Ideal.RO.m{1} Upper.BIRO.IRO'.mp{2}
       ==> ={res}
-          /\ relation Lower.Ideal.RO.m{1} Upper.BIRO.IRO.mp{2}.
+          /\ lower Lower.Ideal.RO.m{1} Upper.BIRO.IRO'.mp{2}.
   proof.
   proc. sp; if=> //=.
-  inline Lower.BlockSponge(Lower.Perm.Perm).f.
+  inline Lower.BlockSponge(Perm).f.
   admit. (* Fun with loops *)
   qed.
 
-print Upper.RealIndif.
+  pred upper (ro : (block list,block) fmap) (iro : (block list * int,block) fmap) =
+    (forall x y, valid_lower x => ro.[x] = Some y => iro.[strip x] = Some y)
+    /\ (forall x n y,
+          valid_upper x =>
+          iro.[(x,n)] = Some y =>
+          exists n',
+               n <= n'
+            /\ mem (dom ro) (extend x n')).
+
+  module LowIRO' : Lower.FUNCTIONALITY = {
+    proc init = Upper.BIRO.IRO'.init
+    proc f(x : block list) = {
+      var b <- b0;
+
+      if (valid_lower x) {
+        b <@ Upper.BIRO.IRO'.f_lazy(strip x);
+      }
+
+      return b;
+    }
+  }.
+
+  pred holey_map (iro iro_lazy : (block list * int,block) fmap) =
+        Upper.BIRO.prefix_closed iro
+     /\ (forall xn,
+          mem (dom iro_lazy) xn =>
+          iro_lazy.[xn] = iro.[xn])
+     /\ (forall x n,
+          mem (dom iro) (x,n) =>
+          exists n',
+               n <= n'
+            /\ mem (dom iro_lazy) (x,n')).
+
+  (** Essentially, we can delay sampling every entry in the left map
+      whose index is not in the index of the right map, as they have
+      not ben given to the adversary. **)
+  local lemma LazifyIRO:
+    eager [Upper.BIRO.IRO'.resample_invisible(); , LowerFun(Upper.BIRO.IRO').f ~ LowIRO'.f, Upper.BIRO.IRO'.resample_invisible();:
+              ={arg, Upper.BIRO.IRO'.visible}
+           /\ holey_map Upper.BIRO.IRO'.mp{1} Upper.BIRO.IRO'.mp{2}
+           /\ Upper.BIRO.IRO'.visible{2} = dom (Upper.BIRO.IRO'.mp){2}
+           ==>     ={res, Upper.BIRO.IRO'.visible}
+               /\ holey_map Upper.BIRO.IRO'.mp{1} Upper.BIRO.IRO'.mp{2}
+               /\ Upper.BIRO.IRO'.visible{2} = dom (Upper.BIRO.IRO'.mp){2}].
+  proof.
+    eager proc.
+    case (!valid_lower p{1})=> /=.
+      rcondf{1} 3; 1: by auto; inline *; auto; while (true); auto.
+      rcondf{2} 2; 1: by auto.
+      inline *; auto.
+      rcondf{2} 4; 1: by auto; smt.
+      while{1} (   work{1} <= dom (Upper.BIRO.IRO'.mp){1}
+                /\ holey_map Upper.BIRO.IRO'.mp{1} Upper.BIRO.IRO'.mp{2}
+                /\ forall x, mem work{1} x => mem (dom Upper.BIRO.IRO'.mp){1} x /\ !mem (dom Upper.BIRO.IRO'.mp){2} x)
+               (card work{1}).
+        auto; progress.
+        + admit. (* TODO: dto lossless *)
+        + move=> x; rewrite domP in_fsetD in_fsetU !in_fset1.
+          by case (x = pick work{hr})=> //= _ /H1 [->].
+        + smt.
+        + smt.
+        + have [_] [_] /(_ x1 n0 _) //= := H0.
+          move: H5; rewrite domP in_fsetU in_fset1=> [//=|h].
+          by have [->]:= H1 (x1,n0) _; first by rewrite h mem_pick // H2.
+        + move: H5; rewrite domP in_fsetD in_fsetU !in_fset1.
+          by case (x1 = pick work{hr})=> //= _ /H1 [->].
+        + move: H5; rewrite in_fsetD in_fset1.
+          by case (x1 = pick work{hr})=> //= _ /H1 [_ ->].
+        + smt.
+      by auto; smt.
+    rcondt{1} 3; 1: by auto; inline *; auto; while (true); auto.
+    rcondt{2} 2; 1: by auto.
+    inline Upper.BIRO.IRO'.f Upper.BIRO.IRO'.f_lazy.
+    rcondt{1} 8; 1: by auto; inline *; auto; while (true); auto; smt.
+    rcondt{2} 4; 1: by auto; smt.
+    case ((mem (dom Upper.BIRO.IRO'.mp) (strip p)){1} /\ !(mem (dom Upper.BIRO.IRO'.mp) (strip x)){2}).
+      admit. (* this is the bad case where we need to bring down the sampling from resample_invisible *)
+    inline{2} Upper.BIRO.IRO'.resample_invisible.
+    rcondf{2} 9; 1: by auto; inline *; sp; if; auto; smt.
+    seq  1  0: ((((p{1} = x{2} /\ ={Upper.BIRO.IRO'.visible}) /\
+    holey_map Upper.BIRO.IRO'.mp{1} Upper.BIRO.IRO'.mp{2} /\
+    Upper.BIRO.IRO'.visible{2} = dom Upper.BIRO.IRO'.mp{2}) /\
+   valid_lower p{1}) /\
+  ! (mem (dom Upper.BIRO.IRO'.mp{1}) (strip p{1}) /\
+     ! mem (dom Upper.BIRO.IRO'.mp{2}) (strip x{2}))). (* disgusting copy-paste. we need seq* *)
+      admit.
+    splitwhile{1} 8: (i < n0 - 1).
+    rcondt{1} 9.
+      move=> &m; while (0 <= i < n0).
+        by inline*; sp; if; auto; smt.
+      by auto; smt.
+    rcondf{1} 12.
+      move=> &m; seq 8: (i = n0 - 1).
+       * wp; while (0 <= i < n0).
+           by inline*; sp; if; auto; smt.
+         by auto; smt.
+       * inline*; sp; if; auto; smt.
+    admit. (* just pushing the proof through *)
+  qed.
+
+
+  (** This is an eager statement:
+        - on actual queries, the two maps agree;
+        - blocks in the IRO that are just generated on the way
+          to answering actual queries can be resampled. **)
+  (* Lower.Ideal.RO.f ~ LowerFun(Upper.BIRO.IRO).f:
+             ={arg}
+          /\ true
+      ==> ={res}.
+  *)
 
   lemma Intermediate &m:
-    `|Pr[Upper.RealIndif(Upper.Perm.Perm,UpperOfLowerBlockSponge,UpperDist).main() @ &m: res]
+    `|Pr[Upper.RealIndif(Perm,Upper.BlockSponge,UpperDist).main() @ &m :res]
+      - Pr[Upper.IdealIndif(Upper.BIRO.IRO,Sim(LowerSim),UpperDist).main() @ &m: res]|
+    = `|Pr[Upper.RealIndif(Perm,UpperOfLowerBlockSponge,UpperDist).main() @ &m: res]
+        - Pr[Upper.IdealIndif(UpperFun(Lower.Ideal.RO),Sim(LowerSim),UpperDist).main() @ &m: res]|.
+  proof.
+  have ->: Pr[Upper.RealIndif(Perm,UpperOfLowerBlockSponge,UpperDist).main() @ &m: res]
+           = Pr[Upper.RealIndif(Perm,Upper.BlockSponge,UpperDist).main() @ &m :res].
+    byequiv=> //=; proc.
+    call (_:   ={m,mi}(Perm,Perm)
+            /\ (forall x, mem (dom Perm.m){1} x)).
+      by proc; if; auto; smt.
+      by proc; if; auto; smt.
+      (* BUG: arg should be handled much earlier and automatically *)
+      by conseq ModularUpper=> //= &1 &2; case (arg{1}); case (arg{2})=> //=.
+    call (_:     true
+             ==>    ={glob Perm}
+                 /\ (forall x, mem (dom Perm.m){1} x)).
+      admit. (* Do this with an eagerly sampled RP *)
+    (* Now the other initialization is dead code. *)
+    call (_: true ==> true)=> //.
+      by proc; auto.
+  have ->: Pr[Upper.IdealIndif(UpperFun(Lower.Ideal.RO),Sim(LowerSim),UpperDist).main() @ &m: res]
+           = Pr[Upper.IdealIndif(Upper.BIRO.IRO,Sim(LowerSim),UpperDist).main() @ &m: res].
+    byequiv=> //=; proc.
+    call (_: ={glob LowerSim} /\ relation Lower.Ideal.RO.m{1} Upper.BIRO.IRO.mp{2}).
+      proc (relation Lower.Ideal.RO.m{1} Upper.BIRO.IRO.mp{2})=> //=.
+        by proc; sp; if=> //=; call ModularLower; auto.
+      proc (relation Lower.Ideal.RO.m{1} Upper.BIRO.IRO.mp{2})=> //=.
+        by proc; sp; if=> //=; call ModularLower; auto.
+      (* Re-Bug *)
+      by conseq ModularLower=> &1 &2; case (arg{1}); case (arg{2}).
+    inline *; wp; call (_: true)=> //=.
+      by sim.
+    auto; progress [-split]; split=> //=.
+    by split=> x y; rewrite map0P.
+  done.
+  qed.
+
+  lemma Remainder &m:
+    `|Pr[Upper.RealIndif(Perm,UpperOfLowerBlockSponge,UpperDist).main() @ &m: res]
       - Pr[Upper.IdealIndif(UpperFun(Lower.Ideal.RO),Sim(LowerSim),UpperDist).main() @ &m: res]|
-    = `|Pr[Lower.RealIndif(Lower.Perm.Perm,Lower.BlockSponge,Dist(UpperDist)).main() @ &m: res]
-      - Pr[Lower.IdealIndif(Lower.Ideal.RO,LowerSim,Dist(UpperDist)).main() @ &m: res]|.
+    = `|Pr[Lower.RealIndif(Perm,Lower.BlockSponge,Dist(UpperDist)).main() @ &m: res]
+        - Pr[Lower.IdealIndif(Lower.Ideal.RO,LowerSim,Dist(UpperDist)).main() @ &m: res]|.
   proof. admit. qed.
 
   lemma Conclusion &m:
-    `|Pr[Upper.RealIndif(Upper.Perm.Perm,Upper.BlockSponge,UpperDist).main() @ &m: res]
+    `|Pr[Upper.RealIndif(Perm,Upper.BlockSponge,UpperDist).main() @ &m: res]
       - Pr[Upper.IdealIndif(Upper.BIRO.IRO,Sim(LowerSim),UpperDist).main() @ &m: res]|
-    = `|Pr[Lower.RealIndif(Lower.Perm.Perm,Lower.BlockSponge,Dist(UpperDist)).main() @ &m: res]
+    = `|Pr[Lower.RealIndif(Perm,Lower.BlockSponge,Dist(UpperDist)).main() @ &m: res]
       - Pr[Lower.IdealIndif(Lower.Ideal.RO,LowerSim,Dist(UpperDist)).main() @ &m: res]|.
-  proof. admit. qed.
+  proof. by rewrite (Intermediate &m) (Remainder &m). qed.
 end section.
